instructions/binary_search/a0_spec.v
@@ -2,9 +2,9 @@ Require Import isla.isla.
 Require Import isla.aarch64.aarch64.
 Require Export isla.instructions.binary_search.a0.
 
-Lemma a0_spec `{!islaG Σ} `{!threadG}:
-  instr 0x10300000 (Some a0) -∗
-  instr_body 0x10300000 (stp_uninit_spec 0x0000000010300000 "R29" "R30" "SP_EL2" (-64) true).
+Lemma a0_spec `{!islaG Σ} `{!threadG} pc:
+  instr pc (Some a0) -∗
+  instr_body pc (stp_uninit_spec pc "R29" "R30" "SP_EL2" (-64) true).
 Proof.
   iStartProof.
   repeat liAStep; liShow.
@@ -12,6 +12,6 @@ Proof.
   all: bv_solve.
 Qed.
 
-Definition a0_spec_inst `{!islaG Σ} `{!threadG} :=
-  entails_to_simplify_hyp 0 a0_spec.
+Definition a0_spec_inst `{!islaG Σ} `{!threadG} pc :=
+  entails_to_simplify_hyp 0 (a0_spec pc).
 Global Existing Instance a0_spec_inst.
