instructions/binary_search/a48_spec.v
@@ -2,9 +2,9 @@ Require Import isla.isla.
 Require Import isla.aarch64.aarch64.
 Require Export isla.instructions.binary_search.a48.
 
-Lemma a48_spec `{!islaG Σ} `{!threadG}:
-  instr 0x10300048 (Some a48) -∗
-  instr_body 0x10300048 (csinc_spec 0x0000000010300048 "R23" "R24").
+Lemma a48_spec `{!islaG Σ} `{!threadG} pc:
+  instr pc (Some a48) -∗
+  instr_body pc (csinc_spec pc "R23" "R24").
 Proof.
   iStartProof.
   repeat liAStep; liShow.
@@ -12,6 +12,6 @@ Proof.
   all: csinc_spec_tac.
 Qed.
 
-Definition a48_spec_inst `{!islaG Σ} `{!threadG} :=
-  entails_to_simplify_hyp 0 a48_spec.
+Definition a48_spec_inst `{!islaG Σ} `{!threadG} pc :=
+  entails_to_simplify_hyp 0 (a48_spec pc).
 Global Existing Instance a48_spec_inst.
