instructions/binary_search/a4c_spec.v
@@ -2,9 +2,9 @@ Require Import isla.isla.
 Require Import isla.aarch64.aarch64.
 Require Export isla.instructions.binary_search.a4c.
 
-Lemma a4c_spec `{!islaG Σ} `{!threadG}:
-  instr 0x1030004c (Some a4c) -∗
-  instr_body 0x1030004c (cmp_R_R_spec 0x000000001030004c "R20" "R23").
+Lemma a4c_spec `{!islaG Σ} `{!threadG} pc:
+  instr pc (Some a4c) -∗
+  instr_body pc (cmp_R_R_spec pc "R20" "R23").
 Proof.
   iStartProof.
   repeat liAStep; liShow.
@@ -12,6 +12,6 @@ Proof.
   1: cmp_spec_tac1. 1: cmp_spec_tac2. 1: cmp_spec_tac3. 1: cmp_spec_tac4.
 Qed.
 
-Definition a4c_spec_inst `{!islaG Σ} `{!threadG} :=
-  entails_to_simplify_hyp 0 a4c_spec.
+Definition a4c_spec_inst `{!islaG Σ} `{!threadG} pc :=
+  entails_to_simplify_hyp 0 (a4c_spec pc).
 Global Existing Instance a4c_spec_inst.
