instructions/binary_search/a60_spec.v
@@ -2,9 +2,9 @@ Require Import isla.isla.
 Require Import isla.aarch64.aarch64.
 Require Export isla.instructions.binary_search.a60.
 
-Lemma a60_spec `{!islaG Σ} `{!threadG}:
-  instr 0x10300060 (Some a60) -∗
-  instr_body 0x10300060 (ldp_mapsto_spec 0x0000000010300060 "R20" "R19" "SP_EL2" (48) None).
+Lemma a60_spec `{!islaG Σ} `{!threadG} pc:
+  instr pc (Some a60) -∗
+  instr_body pc (ldp_mapsto_spec pc "R20" "R19" "SP_EL2" (48) None).
 Proof.
   iStartProof.
   repeat liAStep; liShow.
@@ -12,6 +12,6 @@ Proof.
   all: bv_solve.
 Qed.
 
-Definition a60_spec_inst `{!islaG Σ} `{!threadG} :=
-  entails_to_simplify_hyp 0 a60_spec.
+Definition a60_spec_inst `{!islaG Σ} `{!threadG} pc :=
+  entails_to_simplify_hyp 0 (a60_spec pc).
 Global Existing Instance a60_spec_inst.
