instructions/binary_search/a68_spec.v
@@ -2,12 +2,12 @@ Require Import isla.isla.
 Require Import isla.aarch64.aarch64.
 Require Export isla.instructions.binary_search.a68.
 
-Lemma a68_spec `{!islaG Σ} `{!threadG}:
-  instr 0x10300068 (Some a68) -∗
-  instr_body 0x10300068 (ldp_mapsto_spec 0x0000000010300068 "R24" "R23" "SP_EL2" (16) None).
+Lemma a68_spec `{!islaG Σ} `{!threadG} pc:
+  instr pc (Some a68) -∗
+  instr_body pc (ldp_mapsto_spec pc "R24" "R23" "SP_EL2" (16) None).
 Proof.
 Admitted.
 
-Definition a68_spec_inst `{!islaG Σ} `{!threadG} :=
-  entails_to_simplify_hyp 0 a68_spec.
+Definition a68_spec_inst `{!islaG Σ} `{!threadG} pc :=
+  entails_to_simplify_hyp 0 (a68_spec pc).
 Global Existing Instance a68_spec_inst.
