instructions/binary_search/a6c_spec.v
@@ -2,12 +2,12 @@ Require Import isla.isla.
 Require Import isla.aarch64.aarch64.
 Require Export isla.instructions.binary_search.a6c.
 
-Lemma a6c_spec `{!islaG Σ} `{!threadG}:
-  instr 0x1030006c (Some a6c) -∗
-  instr_body 0x1030006c (ldp_mapsto_spec 0x000000001030006c "R29" "R30" "SP_EL2" (0) (Some 64)).
+Lemma a6c_spec `{!islaG Σ} `{!threadG} pc:
+  instr pc (Some a6c) -∗
+  instr_body pc (ldp_mapsto_spec pc "R29" "R30" "SP_EL2" (0) (Some 64)).
 Proof.
 Admitted.
 
-Definition a6c_spec_inst `{!islaG Σ} `{!threadG} :=
-  entails_to_simplify_hyp 0 a6c_spec.
+Definition a6c_spec_inst `{!islaG Σ} `{!threadG} pc :=
+  entails_to_simplify_hyp 0 (a6c_spec pc).
 Global Existing Instance a6c_spec_inst.
