instructions/binary_search/a74_spec.v
@@ -2,9 +2,9 @@ Require Import isla.isla.
 Require Import isla.aarch64.aarch64.
 Require Export isla.instructions.binary_search.a74.
 
-Lemma a74_spec `{!islaG Σ} `{!threadG}:
-  instr 0x10300074 (Some a74) -∗
-  instr_body 0x10300074 (cmp_R_R_spec 0x0000000010300074 "R0" "R1").
+Lemma a74_spec `{!islaG Σ} `{!threadG} pc:
+  instr pc (Some a74) -∗
+  instr_body pc (cmp_R_R_spec pc "R0" "R1").
 Proof.
   iStartProof.
   repeat liAStep; liShow.
@@ -12,6 +12,6 @@ Proof.
   1: cmp_spec_tac1. 1: cmp_spec_tac2. 1: cmp_spec_tac3. 1: cmp_spec_tac4.
 Qed.
 
-Definition a74_spec_inst `{!islaG Σ} `{!threadG} :=
-  entails_to_simplify_hyp 0 a74_spec.
+Definition a74_spec_inst `{!islaG Σ} `{!threadG} pc :=
+  entails_to_simplify_hyp 0 (a74_spec pc).
 Global Existing Instance a74_spec_inst.
