instructions/binary_search/ac_spec.v
@@ -2,12 +2,12 @@ Require Import isla.isla.
 Require Import isla.aarch64.aarch64.
 Require Export isla.instructions.binary_search.ac.
 
-Lemma ac_spec `{!islaG Σ} `{!threadG}:
-  instr 0x1030000c (Some ac) -∗
-  instr_body 0x1030000c (stp_uninit_spec 0x000000001030000c "R20" "R19" "SP_EL2" (48) false).
+Lemma ac_spec `{!islaG Σ} `{!threadG} pc:
+  instr pc (Some ac) -∗
+  instr_body pc (stp_uninit_spec pc "R20" "R19" "SP_EL2" (48) false).
 Proof.
 Admitted.
 
-Definition ac_spec_inst `{!islaG Σ} `{!threadG} :=
-  entails_to_simplify_hyp 0 ac_spec.
+Definition ac_spec_inst `{!islaG Σ} `{!threadG} pc :=
+  entails_to_simplify_hyp 0 (ac_spec pc).
 Global Existing Instance ac_spec_inst.
