instructions/riscv64_test/a8_spec.v
@@ -2,9 +2,9 @@ Require Import isla.isla.
 Require Import isla.riscv64.riscv64.
 Require Export isla.instructions.riscv64_test.a8.
 
-Lemma a8_spec `{!islaG Σ} `{!threadG}:
-  instr 0x10300008 (Some a8) -∗
-  instr_body 0x10300008 (sd_spec 0x0000000010300008 "x11" "x2" (8)).
+Lemma a8_spec `{!islaG Σ} `{!threadG} pc:
+  instr pc (Some a8) -∗
+  instr_body pc (sd_spec pc "x11" "x2" (8)).
 Proof.
   iStartProof.
   repeat liAStep; liShow.
@@ -12,6 +12,6 @@ Proof.
   all: bv_solve.
 Qed.
 
-Definition a8_spec_inst `{!islaG Σ} `{!threadG} :=
-  entails_to_simplify_hyp 0 a8_spec.
+Definition a8_spec_inst `{!islaG Σ} `{!threadG} pc :=
+  entails_to_simplify_hyp 0 (a8_spec pc).
 Global Existing Instance a8_spec_inst.
